path for slices

proof/correctness/avx2/MLKEM_InnerPKE_avx2.ec
@@ -1815,8 +1815,12 @@ rewrite BVA_Top_Array1088_Array1088_t.tolistP.
 apply eq_in_mkseq => i i_bnd; smt(Array1088.initE).
 qed.
 
-op sliceget256_16_256 (arr: W16.t Array256.t) (offset: int) : W256.t =  W256.bits2w (take 256 (drop offset (flatten (map W16.w2bits (Array256.to_list arr))))).
+op sliceget256_16_256 (arr: W16.t Array256.t) (offset: int) : W256.t = 
+   if 8 %| offset then 
+    get256_direct ((init16 (fun (i_0 : int) => arr.[i_0])))%WArray512 (offset %/ 8)
+   else W256.bits2w (take 256 (drop offset (flatten (map W16.w2bits (to_list arr))))).
 
+(*
 lemma flatten_take_drop_16  (l : W16.t list) (csize offset bit : int) :
   0 <= offset =>
   offset + csize <= 16 * size l =>
@@ -1833,13 +1837,6 @@ rewrite -get_w2bits;congr.
 by rewrite (nth_map witness) 1:/#. 
 qed.
 
-lemma size_flatten_W16_w2bits (a : W16.t list) :
-  (size (flatten (map W16.w2bits (a))))  =  16 * size a.
-proof.
-  rewrite size_flatten -map_comp /(\o) /=.
-  rewrite StdBigop.Bigint.sumzE /= StdBigop.Bigint.BIA.big_mapT /(\o) /=. 
-  rewrite StdBigop.Bigint.big_constz count_predT /#.
-qed.
 
 lemma aligned_get256_16_256 arr offset :
 0 <= offset <= 16*256 - 256 =>
@@ -1856,20 +1853,29 @@ rewrite get_bits8 1:/#.
 smt(@IntDiv). 
 qed.
 
-
+*)
 bind op [W16.t & W256.t & Array256.t] sliceget256_16_256 "asliceget".
 realize bvaslicegetP.
-move => *; rewrite /sliceget256_16_256 bits2wK // size_take //= size_drop //=.
-admit. (* bounds are incomplete! 0 <= offset <= 16 * 256 - 256 *)
-by smt(Array256.size_to_list size_flatten_W16_w2bits).
+
+move => /= arr offset; rewrite /sliceget256_16_256 /= => H k kb. 
+case (8%| offset) => /= *; last by smt(W256.get_bits2w).
+rewrite /get256_direct pack32E initiE 1:/# /= initiE 1:/# /= initiE 1:/# /= bits8E initiE 1:/# /=.
+rewrite nth_take 1,2:/# nth_drop 1,2:/#.
+rewrite (BitEncoding.BitChunking.nth_flatten false 16 _). 
++ rewrite allP => x /=; rewrite mapP => He; elim He;smt(W16.size_w2bits).
+rewrite (nth_map W16.zero []); 1: smt(Array256.size_to_list).
+by rewrite nth_mkseq /#.
 qed.
 
 import BitEncoding BS2Int BitChunking.
 
-op sliceset256_16_256 (arr: W16.t Array256.t) (offset: int) (bv: W256.t) : W16.t Array256.t = Array256.of_list witness (map W16.bits2w (chunk 16 (take offset (flatten (map W16.w2bits (to_list arr))) ++ w2bits bv ++
+op sliceset256_16_256 (arr: W16.t Array256.t) (offset: int) (bv: W256.t) : W16.t Array256.t =
+  if 8 %| offset
+  then (init (fun (i3 : int) => get16 (set256_direct ((init16 (fun (i_0 : int) => arr.[i_0])))%WArray512 (offset %/ 8) bv) i3))%Array256
+  else  Array256.of_list witness (map W16.bits2w (chunk 16 (take offset (flatten (map W16.w2bits (to_list arr))) ++ w2bits bv ++
   drop (offset + 256) (flatten (map W16.w2bits (to_list arr)))))).
 
-
+(*
 lemma aligned_set256_16_256 arr offset bv :
 0 <= offset <= 16*256 - 256 =>
 256 %| offset  => 
@@ -1930,24 +1936,41 @@ case (2 * i < 32 * (offset %/ 256 + 1));last first.
    rewrite nth_drop; 1,2: by smt(size_take size_drop  W16.size_w2bits size_cat Array256.size_to_list size_flatten_W16_w2bits size_ge0). 
    rewrite !get_w2bits get_bits16;by smt(size_take size_drop  W16.size_w2bits size_cat Array256.size_to_list size_flatten_W16_w2bits size_ge0). 
 qed.
+*)
 
-
+lemma size_flatten_W16_w2bits (a : W16.t list) :
+  (size (flatten (map W16.w2bits (a))))  =  16 * size a.
+proof.
+  rewrite size_flatten -map_comp /(\o) /=.
+  rewrite StdBigop.Bigint.sumzE /= StdBigop.Bigint.BIA.big_mapT /(\o) /=. 
+  rewrite StdBigop.Bigint.big_constz count_predT /#.
+qed.
 
 bind op [W16.t & W256.t & Array256.t] sliceset256_16_256 "asliceset".
-realize bvaslicesetP.  (* bounds are incomplete! 0 <= offset <= 16 * 256 - 256 *)
-move => arr offset bv *. have ? : 0 <= offset by admit.
-rewrite /sliceset256_16_256 of_listK.
-+ rewrite size_map size_chunk // !size_cat size_take 1:/#.
-  by smt(size_take size_drop  W16.size_w2bits size_cat Array256.size_to_list size_flatten_W16_w2bits size_ge0). 
-rewrite -(map_comp W16.w2bits W16.bits2w) /(\o). 
-have := eq_in_map ((fun (x : bool list) => w2bits ((bits2w x))%W16)) idfun (chunk 16
+realize bvaslicesetP. 
+move => arr offset bv H /= k kb; rewrite /sliceset256_16_256 /=. 
+case (8 %| offset) => /= *; last first.
++ rewrite of_listK; 1: by rewrite size_map size_chunk // !size_cat size_take;
+      by smt(size_take size_drop  W16.size_w2bits size_cat Array256.size_to_list size_flatten_W16_w2bits size_ge0). 
+  rewrite -(map_comp W16.w2bits W16.bits2w) /(\o). 
+  have := eq_in_map ((fun (x : bool list) => w2bits ((bits2w x))%W16)) idfun (chunk 16
         (take offset (flatten (map W16.w2bits (to_list arr))) ++ w2bits bv ++
          drop (offset + 256) (flatten (map W16.w2bits (to_list arr))))).
-rewrite iffE => [#] -> * /=. 
-+ by smt(in_chunk_size W16.bits2wK).
-rewrite map_id /= chunkK //.
-+ rewrite !size_cat size_take 1:/#.
-  by smt(size_take size_drop  W16.size_w2bits size_cat Array256.size_to_list size_flatten_W16_w2bits size_ge0). 
+  rewrite iffE => [#] -> * /=; 1: by smt(in_chunk_size W16.bits2wK).
+  rewrite map_id /= chunkK //;1: by rewrite !size_cat size_take;
+    by smt(size_take size_drop  W16.size_w2bits size_cat Array256.size_to_list size_flatten_W16_w2bits size_ge0). 
+  by rewrite !nth_cat !size_cat /=;
+     smt(nth_take nth_drop size_take size_drop  W16.size_w2bits size_cat Array256.size_to_list size_flatten_W16_w2bits size_ge0). 
+rewrite (nth_flatten _ 16); 1: by rewrite allP => i;rewrite mapP => He; elim He;smt(W16.size_w2bits).
+rewrite (nth_map W16.zero []); 1: smt(Array256.size_to_list).
+rewrite nth_mkseq 1:/# /= initiE 1:/# /= get16E pack2E initiE 1:/# /= initiE 1:/# /= /set256_direct.
+rewrite initiE 1:/# /=.
+case (offset <= k && k < offset + 256) => *; 1: by 
+  rewrite ifT 1:/#  get_bits8 /= 1,2:/# initiE // initiE //.
+rewrite ifF 1:/# initiE 1:/# /=.
+rewrite (nth_flatten _ 16); 1: by rewrite allP => i;rewrite mapP => He; elim He;smt(W16.size_w2bits).
+rewrite (nth_map W16.zero []); 1: smt(Array256.size_to_list).
+rewrite nth_mkseq 1:/# /= bits8E /= initiE /# /=.
 qed.
 
 op sliceget32_8_256 (arr: W8.t Array32.t) (i: int) : W256.t = get256 (WArray32.init8 (fun (i_0 : int) => pvc_shufbidx_s.[i_0])) (i%/256).
@@ -2386,36 +2409,24 @@ proc.
 inline *.
 proc change 1 : (init_1088_8 (fun i => W8.zero));1: by auto. 
 proc change 3 : (init_256_16 (fun i => r.[i]));1: by auto.
-proc change ^while.1 : (sliceget256_16_256 ap (i0*256)). 
-   move => &hr; rewrite aligned_get256_16_256; 2..: by smt(). admit. (* We need a loop invariant *)
-proc change ^while.11 : (sliceset256_16_256 ap (i0*256) a1). 
-   move => &hr; rewrite aligned_set256_16_256;2..: by smt().  admit. (* We need a loop invariant *)
+proc change ^while.1 : (sliceget256_16_256 ap (i0*256)); 1: by smt().
+proc change ^while.11 : (sliceset256_16_256 ap (i0*256) a1);1 : by smt(). 
 
 proc change 10 : (init_768_16 (fun i => if 0 <= i && i < 256 then aux.[i] else r.[i]));1: by auto.
 proc change 11 : (init_256_16 (fun i => r.[256 + i]));1: by auto.
-
-proc change ^while{2}.1 : (sliceget256_16_256 ap0 (i1*256)).
-   move => &hr; rewrite aligned_get256_16_256; 2..: by smt(). admit. (* We need a loop invariant *)
-
-proc change ^while{2}.11 : (sliceset256_16_256 ap0 (i1*256) a2).
-   move => &hr; rewrite aligned_set256_16_256;2..: by smt().  admit. (* We need a loop invariant *)
-
+proc change ^while{2}.1 : (sliceget256_16_256 ap0 (i1*256)); 1: by smt().
+proc change ^while{2}.11 : (sliceset256_16_256 ap0 (i1*256) a2);1: by smt().
 
 proc change 18 : (init_768_16 (fun i => if 256 <= i && i < 256 + 256 then aux.[i - 256] else r.[i]));1: by auto.
 proc change 19 : (init_256_16 (fun i => r.[2*256 + i]));1: by auto.
-proc change ^while{3}.1 : (sliceget256_16_256 ap1 (i2*256)).
-   move => &hr; rewrite aligned_get256_16_256;2..: by smt().  admit. (* We need a loop invariant *)
-
-proc change ^while{3}.11 : (sliceset256_16_256 ap1 (i2*256) a3).
-   move => &hr; rewrite aligned_set256_16_256;2..: by smt().  admit. (* We need a loop invariant *)
+proc change ^while{3}.1 : (sliceget256_16_256 ap1 (i2*256)); 1: by smt().
+proc change ^while{3}.11 : (sliceset256_16_256 ap1 (i2*256) a3); 1: by smt().
 
 proc change 26 : (init_768_16 (fun i => if 2 * 256 <= i < 3 * 256 then aux.[i - 2 * 256] else r.[i]));1: by auto.
-
 proc change 30 : (init_960_8 (fun i_0 => ctp0.[i_0 + 0]));1: by done.
 proc change 37 : (sliceget32_8_256 pvc_shufbidx_s 0);1: by auto.
 
 proc change ^while{4}.1 : (sliceget768_16_256 a (i*256));1: by smt().
-
 proc change ^while{4}.25 : (sliceset960_8_128 rp (i * 160) lo); 1: by smt().
 proc change ^while{4}.26 : (sliceset960_8_32 rp (i * 160 + 128) (VPEXTR_32 hi W8.zero));1: by smt().
 cfold 38.
